theory/ComplexityR0.dfy
@@ -1,5 +1,5 @@
-include "./math/ExpNat.dfy"
-include "./math/Misc.dfy"
+include "./math/ExpReal.dfy"
+include "./math/LemFunction.dfy"
 include "./math/TypeR0.dfy"
 
 /**************************************************************************
@@ -7,23 +7,28 @@ include "./math/TypeR0.dfy"
 **************************************************************************/
 
 module ComplexityR0 { 
-  import opened ExpNat   
-  import opened Misc 
+  import opened ExpReal
+  import opened LemFunction 
   import opened TypeR0 
 
-  ghost predicate bigOR0(f:nat->R0, g:nat->R0)
+  ghost predicate bigO(f:nat->R0, g:nat->R0)
   { 
-    exists c:R0, n0:nat :: bigOR0from(c, n0, f, g) 
+    exists c:R0, n0:nat :: bigOfrom(c, n0, f, g) 
   }
 
-  ghost predicate bigOR0from(c:R0, n0:nat, f:nat->R0, g:nat->R0)
+  ghost predicate bigOfrom(c:R0, n0:nat, f:nat->R0, g:nat->R0)
   {
     forall n:nat :: 0 <= n0 <= n ==> f(n) <= c*g(n)
   }
 
-  ghost predicate tIsBigOR0(n:nat, t:R0, g:nat->R0)
+  ghost predicate tIsBigO(n:nat, t:R0, g:nat->R0)
   { 
-    exists f:nat->R0 :: t <= f(n) && bigOR0(f,g)
+    exists f:nat->R0 :: t <= f(n) && bigO(f,g)
+  }
+
+  ghost predicate isBigOPoly(f:nat->R0)
+  { 
+    exists k:R0 :: bigO(f, n => pow(n as R0, k))
   }
 
   /**************************************************************************
@@ -32,72 +37,72 @@ module ComplexityR0 {
 
   // Reflexivity
   // f ∈ O(f)
-  lemma lem_bigOR0_refl(f:nat->R0)  
-    ensures bigOR0(f, f) 
+  lemma lem_bigO_refl(f:nat->R0)  
+    ensures bigO(f, f) 
   {  
     // we show that c=1.0 and n0=0
     assert forall n:nat :: 0 <= 0 <= n ==> f(n) <= 1.0*f(n);
-    assert bigOR0from(1.0, 0, f, f);
+    assert bigOfrom(1.0, 0, f, f);
   }
 
   // If f ∈ O(g) and a>0 then a*f ∈ O(g)
-  lemma lem_bigOR0_constFactor(f:nat->R0, g:nat->R0, a:R0)  
-    requires bigOR0(f, g) 
+  lemma lem_bigO_constFactor(f:nat->R0, g:nat->R0, a:R0)  
+    requires bigO(f, g) 
     requires a > 0.0 
-    ensures  bigOR0(n => a*f(n), g) 
+    ensures  bigO(n => a*f(n), g) 
   {  
-    var c:R0, n0:nat :| bigOR0from(c, n0, f, g);  
+    var c:R0, n0:nat :| bigOfrom(c, n0, f, g);  
     assert forall n:nat :: 0 <= n0 <= n ==> f(n) <= c*g(n);
     
     // we show that c'=a*c and n0'=n0
     assert forall n:nat :: 0 <= n0 <= n ==> a*f(n) <= (a*c)*g(n);
-    assert bigOR0from(a*c, n0, n => a*f(n), g);
+    assert bigOfrom(a*c, n0, n => a*f(n), g);
   }
 
   // If f1 ∈ O(g1) and f2 ∈ O(g2) then f1+f2 ∈ O(g1+g2)
-  lemma lem_bigOR0_sum(f1:nat->R0, g1:nat->R0, f2:nat->R0, g2:nat->R0)  
-    requires bigOR0(f1, g1) 
-    requires bigOR0(f2, g2) 
-    ensures  bigOR0(n => f1(n)+f2(n), n => g1(n)+g2(n)) 
+  lemma lem_bigO_sum(f1:nat->R0, g1:nat->R0, f2:nat->R0, g2:nat->R0)  
+    requires bigO(f1, g1) 
+    requires bigO(f2, g2) 
+    ensures  bigO(n => f1(n)+f2(n), n => g1(n)+g2(n)) 
   {  
-    var c1:R0, n1:nat :| bigOR0from(c1, n1, f1, g1);  
+    var c1:R0, n1:nat :| bigOfrom(c1, n1, f1, g1);  
     assert forall n:nat :: 0 <= n1 <= n ==> f1(n) <= c1*g1(n);
-    var c2:R0, n2:nat :| bigOR0from(c2, n2, f2, g2);  
+    var c2:R0, n2:nat :| bigOfrom(c2, n2, f2, g2);  
     assert forall n:nat :: 0 <= n2 <= n ==> f2(n) <= c2*g2(n);   
     
     // we show that c=c1+c2 and n0=n1+n2
     assert forall n:nat :: 0 <= n1+n2 <= n ==> f1(n) + f2(n) <= c1*g1(n) + c2*g2(n);
     assert forall n:nat :: 0 <= n1+n2 <= n ==> f1(n) + f2(n) <= (c1+c2)*(g1(n) + g2(n));
-    assert bigOR0from(c1+c2, n1+n2, n => f1(n)+f2(n), n => g1(n)+g2(n));
+    assert bigOfrom(c1+c2, n1+n2, n => f1(n)+f2(n), n => g1(n)+g2(n));
   }
 
   // If f1 ∈ O(g1) and f2 ∈ O(g2) then f1*f2 ∈ O(g1*g2)
-  lemma lem_bigOR0_prod(f1:nat->R0, g1:nat->R0, f2:nat->R0, g2:nat->R0)  
-    requires bigOR0(f1, g1) 
-    requires bigOR0(f2, g2) 
-    ensures  bigOR0(n => f1(n)*f2(n), n => g1(n)*g2(n)) 
+  lemma lem_bigO_prod(f1:nat->R0, g1:nat->R0, f2:nat->R0, g2:nat->R0)  
+    requires bigO(f1, g1) 
+    requires bigO(f2, g2) 
+    ensures  bigO(n => f1(n)*f2(n), n => g1(n)*g2(n)) 
   {  
-    var c1:R0, n1:nat :| bigOR0from(c1, n1, f1, g1);  
+    var c1:R0, n1:nat :| bigOfrom(c1, n1, f1, g1);  
     assert forall n:nat :: 0 <= n1 <= n ==> f1(n) <= c1*g1(n);
-    var c2:R0, n2:nat :| bigOR0from(c2, n2, f2, g2);  
+    var c2:R0, n2:nat :| bigOfrom(c2, n2, f2, g2);  
     assert forall n:nat :: 0 <= n2 <= n ==> f2(n) <= c2*g2(n);   
     
     // we show that c=c1*c2 and n0=n1+n2
     assert forall n:nat :: 0 <= n1+n2 <= n ==> f1(n)*f2(n) <= (c1*g1(n))*(c2*g2(n));
     assert forall n:nat :: 0 <= n1+n2 <= n ==> f1(n)*f2(n) <= (c1*c2)*(g1(n)*g2(n));
-    assert bigOR0from(c1*c2, n1+n2, n => f1(n)*f2(n), n => g1(n)*g2(n));
+    assert bigOfrom(c1*c2, n1+n2, n => f1(n)*f2(n), n => g1(n)*g2(n));
   }
 
   // Transitivity
   // If f ∈ O(g) and g ∈ O(h) then f ∈ O(h)
-  lemma lem_bigOR0_trans(f:nat->R0, g:nat->R0, h:nat->R0)  
-    requires bigOR0(f, g) 
-    requires bigOR0(g, h) 
-    ensures  bigOR0(f, h) 
+  lemma lem_bigO_trans(f:nat->R0, g:nat->R0, h:nat->R0)  
+    requires bigO(f, g) 
+    requires bigO(g, h) 
+    ensures  bigO(f, h) 
   {  
-    var c1:R0, n1:nat :| bigOR0from(c1, n1, f, g);  
+    var c1:R0, n1:nat :| bigOfrom(c1, n1, f, g);  
     assert forall n:nat :: 0 <= n1 <= n ==> f(n) <= c1*g(n);
-    var c2:R0, n2:nat :| bigOR0from(c2, n2, g, h);  
+    var c2:R0, n2:nat :| bigOfrom(c2, n2, g, h);  
     assert forall n:nat :: 0 <= n2 <= n ==> g(n) <= c2*h(n);   
     
     // we show that c=c1*c2 and n0=n1+n2
@@ -106,15 +111,14 @@ module ComplexityR0 {
     {
       if 0 <= n1+n2 <= n {
         calc {
-            f(n); 
-          <=
-            c1*g(n);
+             f(n); 
+          <= c1*g(n);
           <= { assert g(n) <= c2*h(n); } 
-            c1*c2*h(n);         
+             c1*c2*h(n);         
         }
       }
     }
-    assert bigOR0from(c1*c2, n1+n2, f, h);
+    assert bigOfrom(c1*c2, n1+n2, f, h);
   }
 
   // TODO: prove If f ∈ O(g) then f+g ∈ O(g)
