theory/masterLR.dfy
@@ -4,8 +4,7 @@ include "./math/FloorCeil.dfy"
 include "./math/LemBoundsNat.dfy"
 include "./math/LemFunction.dfy"
 include "./math/MaxMin.dfy"
-include "./math/Misc.dfy"
-include "./math/SummationReal.dfy"
+include "./math/SumReal.dfy"
 include "./math/TypeR0.dfy"
 include "./ComplexityR0.dfy"
 
@@ -14,11 +13,9 @@ module MasterLR {
   import opened FloorCeil   
   import opened LemBoundsNat
   import opened LemFunction
-  import opened MaxMin 
-  import opened Misc 
-  import opened SummationReal
+  import opened MaxMin
+  import opened SumReal
   import opened TypeR0 
-
   import opened ComplexityR0
 
   // Following recurrence models a recursive computation where
@@ -46,13 +43,13 @@ module MasterLR {
   //         thight Θ(n^k*a^{n/s}) bound when a>1.
   //       In general, we can only be sure of O type bounds. Thigher Θ bounds
   //       require a case by case analysis.
-  lemma {:axiom} thm_masterMethodLR(a:nat, b:nat, c:R0, s:nat, T:nat->R0, w:nat->R0, k:R0)  
+  lemma thm_masterMethodLR(a:nat, b:nat, c:R0, s:nat, T:nat->R0, w:nat->R0, k:R0)
     requires a > 0 && s > 0 && b >= s-1
-    requires bigOR0(w, n => powr(n as R0, k)) 
+    requires bigO(w, n => pow(n as R0, k)) 
     requires forall n:nat :: T(n) == TbodyLR(a, b, c, s, T, w, n) 
 
-    ensures a == 1 ==> bigOR0(T, (n:nat) => powr(n as R0, k + 1.0))
-    ensures a > 1  ==> bigOR0(T, (n:nat) => powr(n as R0, k)*powr(a as R0, (n/s) as R0))
+    ensures a == 1 ==> bigO(T, (n:nat) => pow(n as R0, k + 1.0))
+    ensures a > 1  ==> bigO(T, (n:nat) => pow(n as R0, k)*pow(a as R0, (n/s) as R0))
   {
     // 1. Prove: ∀ n : T(n) = a^m*c + S(n) where m=ceil((n-b)/s)
     assert forall n:nat :: T(n) == TsumForm(a, b, c, s, w, n)
@@ -74,6 +71,7 @@ module MasterLR {
   //      
   //     assert bigOR0(T, (n:nat) => powr(n as R0, k)*powr(a as R0, (n/s) as R0));
     }
+    // TODO
     assert false;
   }
 
@@ -96,20 +94,20 @@ module MasterLR {
   opaque ghost function TsumForm(a:nat, b:nat, c:R0, s:nat, w:nat->R0, n:nat) : real
     requires s > 0
   {    
-    powr(a as R0, m(b,s,n) as real)*c + S(a, b, s, w, n)    
+    pow(a as R0, m(b,s,n) as real)*c + S(a, b, s, w, n)    
   } 
 
   // Expression: sum_{i=0}^{m-1}a^i*w(n-i*s)
   opaque ghost function S(a:nat, b:nat, s:nat, w:nat->R0, n:nat) : real
     requires s > 0
   {    
-    sumr(0, m(b,s,n)-1, i => S1(a,i)*S2(s,w,n,i))      
+    sum(0, m(b,s,n)-1, i => S1(a,i)*S2(s,w,n,i))      
   } 
 
   // Expression: a^i
   opaque ghost function S1(a:nat, i:int) : real
   {    
-    powr(a as R0, i as real)     
+    pow(a as R0, i as real)     
   } 
 
   // Expression: n-i*s
@@ -122,7 +120,7 @@ module MasterLR {
   opaque ghost function SupBound(a:nat, b:nat, s:nat, w:nat->R0, k:R0, n:nat, d:R0) : real
     requires s > 0
   {    
-    d*powr(n as R0, k)*sumr(0, m(b,s,n)-1, i => S1(a,i))    
+    d*pow(n as R0, k)*sum(0, m(b,s,n)-1, i => S1(a,i))    
   } 
 
   // Predicate: ∀ n : S(n) <= SupBound(n,d)
@@ -142,15 +140,15 @@ module MasterLR {
   {
     if n <= b {
       calc {  // ceil((n-b)/s) <= 0
-          ceil(((n-b) as real)/(s as real));
+           ceil(((n-b) as real)/(s as real));
         <= { assert ((n-b) as real)/(s as real) <= 0.0; 
-            lem_ceilxLEQnIFFxLEQn(((n-b) as real)/(s as real),0); }
-          0;
+           lem_ceilxLEQnIFFxLEQn(((n-b) as real)/(s as real),0); }
+           0;
       }  
       calc {
-          m(b,s,n);
+           m(b,s,n);
         == { reveal m(); }
-          max(0, ceil(((n-b) as real)/(s as real)));
+           max(0, ceil(((n-b) as real)/(s as real)));
         == max(0, 0);
         == 0;
       }  
@@ -162,9 +160,9 @@ module MasterLR {
           0;
       }  
       calc {
-          m(b,s,n);
+           m(b,s,n);
         == { reveal m(); }
-          max(0, ceil(((n-b) as real)/(s as real)));
+           max(0, ceil(((n-b) as real)/(s as real)));
         == ceil(((n-b) as real)/(s as real));
       }  
     }
@@ -193,15 +191,15 @@ module MasterLR {
     if n <= b {
       // CB. n <= b
       calc {
-          T(n);
+           T(n);
         == { reveal TbodyLR(); }
-          c;
-        == { lem_mmLR_mValue(b, s, n); reveal S, sumr();  }
-          c + S(a, b, s, w, n);
-        == { lem_mmLR_mValue(b, s, n); lem_powrZero(aR); }
-          powr(aR, mv as real)*c + S(a, b, s, w, n);
+           c;
+        == { lem_mmLR_mValue(b, s, n); reveal S, sum();  }
+           c + S(a, b, s, w, n);
+        == { lem_mmLR_mValue(b, s, n); lem_powZero(aR); }
+           pow(aR, mv as real)*c + S(a, b, s, w, n);
         == { reveal TsumForm(); } 
-          TsumForm(a, b, c, s, w, n);  
+           TsumForm(a, b, c, s, w, n);  
       }      
     } else {
       // Step. n > b
@@ -214,55 +212,55 @@ module MasterLR {
       assert mRewr: mv' == mv - 1 
         by { lem_mmLR_mRewr(a,b,s,n); }
       assert sumRewr:    S(a, b, s, w, n-s) 
-                      == sumr(0, mv-2, i => S1(a,i)*S2(s,w,n,i+1))
+                      == sum(0, mv-2, i => S1(a,i)*S2(s,w,n,i+1))
         by { lem_mmLR_sumRewr(a, b, c, s, T, w, n); }
-      assert sumRewr2:    aR*sumr(0, mv-2, i => S1(a,i)*S2(s,w,n,i+1))
-                      == sumr(0, mv-2, i => S1(a,i+1)*S2(s,w,n,i+1))
+      assert sumRewr2:   aR*sum(0, mv-2, i => S1(a,i)*S2(s,w,n,i+1))
+                      == sum(0, mv-2, i => S1(a,i+1)*S2(s,w,n,i+1))
         by { lem_mmLR_sumRewr2(a, b, c, s, T, w, n); }  
-      assert sumRewr3:    sumr(0, mv-2, i => S1(a,i+1)*S2(s,w,n,i+1))  
-                      == sumr(1, mv-1, i => S1(a,i)*S2(s,w,n,i))
+      assert sumRewr3:   sum(0, mv-2, i => S1(a,i+1)*S2(s,w,n,i+1))  
+                      == sum(1, mv-1, i => S1(a,i)*S2(s,w,n,i))
         by { lem_mmLR_sumRewr3(a, b, c, s, T, w, n); }
       assert wRewr: w(n) == S1(a,0)*S2(s,w,n,0)
         by {
           calc {
-              S1(a,0)*S2(s,w,n,0);
+               S1(a,0)*S2(s,w,n,0);
             == { reveal S2(); } 
-              S1(a,0)*liftD(w,0.0)(n-0*s);
+               S1(a,0)*liftD(w,0.0)(n-0*s);
             == { reveal S1(); } 
-              powr(a as R0, 0 as real)*liftD(w,0.0)(n-0*s); 
-            == { lem_powrZero(a as R0); }    
-              1.0*liftD(w,0.0)(n-0*s); 
-            == { lem_powrZero(a as R0); }    
-              liftD(w,0.0)(n);             
+               pow(a as R0, 0 as real)*liftD(w,0.0)(n-0*s); 
+            == { lem_powZero(a as R0); }    
+               1.0*liftD(w,0.0)(n-0*s); 
+            == { lem_powZero(a as R0); }    
+               liftD(w,0.0)(n);             
           }      
         }  
 
       // Finally, we prove the desired goal
       calc {
-          T(n);
+           T(n);
         == { reveal TbodyLR(); assert n > b; }
-          aR*T(n - s) + w(n); 
+           aR*T(n - s) + w(n); 
         == { lem_mmLR_sumFormInd(a, b, c, s, T, w, n-s); }
-          aR*TsumForm(a, b, c, s, w, n-s) + w(n); 
+           aR*TsumForm(a, b, c, s, w, n-s) + w(n); 
         == { reveal TsumForm(); }
-          aR*(powr(aR, mv' as real)*c + S(a, b, s, w, n-s)) + w(n);  
+           aR*(pow(aR, mv' as real)*c + S(a, b, s, w, n-s)) + w(n);  
         == { reveal mRewr; }
-          aR*(powr(aR, (mv-1) as real)*c + S(a, b, s, w, n-s)) + w(n); 
-        == aR*powr(aR, (mv-1) as real)*c + aR*S(a, b, s, w, n-s) + w(n); 
-        == { lem_powrDef(aR, (mv-1) as real); }
-          powr(aR, mv as real)*c + aR*S(a, b, s, w, n-s) + w(n);     
+           aR*(pow(aR, (mv-1) as real)*c + S(a, b, s, w, n-s)) + w(n); 
+        == aR*pow(aR, (mv-1) as real)*c + aR*S(a, b, s, w, n-s) + w(n); 
+        == { lem_powDef(aR, (mv-1) as real); }
+           pow(aR, mv as real)*c + aR*S(a, b, s, w, n-s) + w(n);     
         == { reveal sumRewr; }
-          powr(aR, mv as real)*c + aR*sumr(0, mv-2, i => S1(a,i)*S2(s,w,n,i+1)) + w(n);
+           pow(aR, mv as real)*c + aR*sum(0, mv-2, i => S1(a,i)*S2(s,w,n,i+1)) + w(n);
         == { reveal sumRewr2; }
-          powr(aR, mv as real)*c + sumr(0, mv-2, i => S1(a,i+1)*S2(s,w,n,i+1)) + w(n);    
+           pow(aR, mv as real)*c + sum(0, mv-2, i => S1(a,i+1)*S2(s,w,n,i+1)) + w(n);    
         == { reveal sumRewr3; }
-          powr(aR, mv as real)*c + sumr(1, mv-1, i => S1(a,i)*S2(s,w,n,i)) + w(n); 
+           pow(aR, mv as real)*c + sum(1, mv-1, i => S1(a,i)*S2(s,w,n,i)) + w(n); 
         == { reveal wRewr; }
-          powr(aR, mv as real)*c + sumr(1, mv-1, i => S1(a,i)*S2(s,w,n,i)) + S1(a,0)*S2(s,w,n,0); 
-        == { reveal sumr(); }
-          powr(aR, mv as real)*c + sumr(0, mv-1, i => S1(a,i)*S2(s,w,n,i));           
+           pow(aR, mv as real)*c + sum(1, mv-1, i => S1(a,i)*S2(s,w,n,i)) + S1(a,0)*S2(s,w,n,0); 
+        == { reveal sum(); }
+           pow(aR, mv as real)*c + sum(0, mv-1, i => S1(a,i)*S2(s,w,n,i));           
         == { reveal TsumForm(), S(); }
-          TsumForm(a, b, c, s, w, n);                                                                   
+           TsumForm(a, b, c, s, w, n);                                                                   
       }  
     } 
   }
@@ -271,20 +269,20 @@ module MasterLR {
     requires a > 0 && s > 0 && b >= s-1
     requires n > b
     requires m(b,s,n) >= 1
-    ensures     sumr(0, m(b,s,n)-2, i => S1(a,i+1)*S2(s,w,n,i+1))  
-            == sumr(1, m(b,s,n)-1, i => S1(a,i)*S2(s,w,n,i))
+    ensures    sum(0, m(b,s,n)-2, i => S1(a,i+1)*S2(s,w,n,i+1))  
+            == sum(1, m(b,s,n)-1, i => S1(a,i)*S2(s,w,n,i))
   {
     var mv := m(b,s,n); assert mv >= 1;
     calc {
-          sumr(0, mv-2, i => S1(a,i+1)*S2(s,w,n,i+1));
-      == { lem_sumr_shiftIndex(0, mv-2, 1, i => S1(a,i+1)*S2(s,w,n,i+1)); } 
-          sumr(1, mv-1, l => (i => S1(a,i+1)*S2(s,w,n,i+1))(l-1)); 
+         sum(0, mv-2, i => S1(a,i+1)*S2(s,w,n,i+1));
+      == { lem_sum_shiftIndex(0, mv-2, 1, i => S1(a,i+1)*S2(s,w,n,i+1)); } 
+         sum(1, mv-1, l => (i => S1(a,i+1)*S2(s,w,n,i+1))(l-1)); 
       == { reveal S2();
-            assert forall l :: 1 <= l <= mv-1 ==> 
-              (i => S1(a,i+1)*S2(s,w,n,i+1))(l-1) == S1(a,l)*S2(s,w,n,l);
-            lem_sumr_leibniz(1, mv-1, l => (i => S1(a,i+1)*S2(s,w,n,i+1))(l-1), 
-                                      l => S1(a,l)*S2(s,w,n,l)); } 
-          sumr(1, mv-1, i => S1(a,i)*S2(s,w,n,i));            
+           assert forall l :: 1 <= l <= mv-1 ==> 
+             (i => S1(a,i+1)*S2(s,w,n,i+1))(l-1) == S1(a,l)*S2(s,w,n,l);
+           lem_sum_leibniz(1, mv-1, l => (i => S1(a,i+1)*S2(s,w,n,i+1))(l-1), 
+                                    l => S1(a,l)*S2(s,w,n,l)); } 
+         sum(1, mv-1, i => S1(a,i)*S2(s,w,n,i));            
     }      
   }
 
@@ -292,29 +290,27 @@ module MasterLR {
     requires a > 0 && s > 0 && b >= s-1
     requires n > b
     requires m(b,s,n) >= 1
-    ensures    (a as R0)*sumr(0, m(b,s,n)-2, i => S1(a,i)*S2(s,w,n,i+1))
-            == sumr(0, m(b,s,n)-2, i => S1(a,i+1)*S2(s,w,n,i+1))
+    ensures    (a as R0)*sum(0, m(b,s,n)-2, i => S1(a,i)*S2(s,w,n,i+1))
+            == sum(0, m(b,s,n)-2, i => S1(a,i+1)*S2(s,w,n,i+1))
   {
     var mv := m(b,s,n); assert mv >= 1;
     var aR := a as R0;
       calc {
-            aR*sumr(0, mv-2, i => S1(a,i)*S2(s,w,n,i+1));
-        == { lem_sumr_linearityConst(0, mv-2, aR, i => S1(a,i)*S2(s,w,n,i+1)); }
-            sumr(0, mv-2, l => aR*(i => S1(a,i)*S2(s,w,n,i+1))(l)); 
+           aR*sum(0, mv-2, i => S1(a,i)*S2(s,w,n,i+1));
+        == { lem_sum_linearityConst(0, mv-2, aR, i => S1(a,i)*S2(s,w,n,i+1)); }
+           sum(0, mv-2, l => aR*(i => S1(a,i)*S2(s,w,n,i+1))(l)); 
         == { reveal S1(); assert aR == a as real;
-            assert forall l :: 
-                0 <= l <= mv-2 ==> 
-                  aR*(i => S1(a,i)*S2(s,w,n,i+1))(l) 
-                  == aR*powr(a as real,l as real)*S2(s,w,n,l+1);
-            lem_sumr_leibniz(0, mv-2, l => aR*(i => S1(a,i)*S2(s,w,n,i+1))(l), 
-                                      l => aR*powr(a as real,l as real)*S2(s,w,n,l+1)); } 
-            sumr(0, mv-2, i => aR*powr(aR,i as real)*S2(s,w,n,i+1));  
-        == { reveal S1(); lem_powrDefAll();
-            assert forall l :: 0 <= l <= mv-2 ==> 
-                aR*powr(aR,l as real)*S2(s,w,n,l+1) == S1(a,l+1)*S2(s,w,n,l+1);
-            lem_sumr_leibniz(0, mv-2, i => aR*powr(aR,i as real)*S2(s,w,n,i+1), 
-                                      i => S1(a,i+1)*S2(s,w,n,i+1)); }       
-            sumr(0, mv-2, i => S1(a,i+1)*S2(s,w,n,i+1));       
+             assert forall l :: 0 <= l <= mv-2 ==> 
+               aR*(i => S1(a,i)*S2(s,w,n,i+1))(l) == aR*pow(a as real,l as real)*S2(s,w,n,l+1);
+             lem_sum_leibniz(0, mv-2, l => aR*(i => S1(a,i)*S2(s,w,n,i+1))(l), 
+                                      l => aR*pow(a as real,l as real)*S2(s,w,n,l+1)); } 
+           sum(0, mv-2, i => aR*pow(aR,i as real)*S2(s,w,n,i+1));  
+        == { reveal S1(); lem_powDefAll();
+             assert forall l :: 0 <= l <= mv-2 ==> 
+               aR*pow(aR,l as real)*S2(s,w,n,l+1) == S1(a,l+1)*S2(s,w,n,l+1);
+             lem_sum_leibniz(0, mv-2, i => aR*pow(aR,i as real)*S2(s,w,n,i+1), 
+                                       i => S1(a,i+1)*S2(s,w,n,i+1)); }       
+           sum(0, mv-2, i => S1(a,i+1)*S2(s,w,n,i+1));       
       }         
   }
 
@@ -322,58 +318,58 @@ module MasterLR {
     requires a > 0 && s > 0 && b >= s-1
     requires n > b
     requires m(b,s,n) >= 1
-    ensures S(a, b, s, w, n-s) == sumr(0, m(b,s,n)-2, i => S1(a,i)*S2(s,w,n,i+1))
+    ensures S(a, b, s, w, n-s) == sum(0, m(b,s,n)-2, i => S1(a,i)*S2(s,w,n,i+1))
   {
     var mv := m(b,s,n); assert mv >= 1;
     calc { 
-          S(a, b, s, w, n-s);
+         S(a, b, s, w, n-s);
       == { reveal S(); lem_mmLR_mRewr(a, b, s, n); }
-          sumr(0, mv-2, i => S1(a,i)*S2(s,w,n-s,i));
+         sum(0, mv-2, i => S1(a,i)*S2(s,w,n-s,i));
       == { reveal S2();
             assert forall i :: 0 <= i <= mv-2 ==> 
               S1(a,i)*S2(s,w,n-s,i) == S1(a,i)*liftD(w,0.0)((n-s)-i*s);
-            lem_sumr_leibniz(0, mv-2, i => S1(a,i)*S2(s,w,n-s,i), 
-                                      i => S1(a,i)*liftD(w,0.0)((n-s)-i*s));  }
-        sumr(0, mv-2, i => S1(a,i)*liftD(w,0.0)((n-s)-i*s)); 
+            lem_sum_leibniz(0, mv-2, i => S1(a,i)*S2(s,w,n-s,i), 
+                                     i => S1(a,i)*liftD(w,0.0)((n-s)-i*s));  }
+         sum(0, mv-2, i => S1(a,i)*liftD(w,0.0)((n-s)-i*s)); 
       == { assert forall i {:trigger S1(a,i), liftD(w,0.0)((n-s)-i*s)} :: 
               0 <= i <= mv-2 ==>     S1(a,i)*liftD(w,0.0)((n-s)-i*s) 
                                   == S1(a,i)*liftD(w,0.0)(n-(i+1)*s);
-            lem_sumr_leibniz(0, mv-2, i => S1(a,i)*liftD(w,0.0)((n-s)-i*s), 
+            lem_sum_leibniz(0, mv-2, i => S1(a,i)*liftD(w,0.0)((n-s)-i*s), 
                                       i => S1(a,i)*liftD(w,0.0)(n-(i+1)*s));  }
-        sumr(0, mv-2, i => S1(a,i)*liftD(w,0.0)((n-(i+1)*s)));  
+         sum(0, mv-2, i => S1(a,i)*liftD(w,0.0)((n-(i+1)*s)));  
       == { reveal S2();
             assert forall i :: 0 <= i <= mv-2 ==> 
               S1(a,i)*liftD(w,0.0)(n-(i+1)*s) == S1(a,i)*S2(s,w,n,i+1);
-            lem_sumr_leibniz(0, mv-2, i => S1(a,i)*liftD(w,0.0)(n-(i+1)*s), 
-                                      i => S1(a,i)*S2(s,w,n,i+1));  }
-        sumr(0, mv-2, i => S1(a,i)*S2(s,w,n,i+1));      
+            lem_sum_leibniz(0, mv-2, i => S1(a,i)*liftD(w,0.0)(n-(i+1)*s), 
+                                     i => S1(a,i)*S2(s,w,n,i+1));  }
+         sum(0, mv-2, i => S1(a,i)*S2(s,w,n,i+1));      
     }  
   }
 
   // m = m' - 1
-  // ceil(((n-s)-b)/s) = m=ceil((n-b)/s) - 1
+  // ceil(((n-s)-b)/s) = ceil((n-b)/s) - 1
   lemma lem_mmLR_mRewr(a:nat, b:nat, s:nat, n:nat)  
     requires a > 0 && s > 0 && b >= s-1
     requires n > b
     requires m(b,s,n) >= 1
     ensures  m(b,s,n-s) == m(b,s,n) - 1
   {
-    assert arith:   (((n-b)-s) as real)/(s as real) 
+    assert arith:  (((n-b)-s) as real)/(s as real) 
                 == ((((n-b) as real)/(s as real)) - ((s/s) as real));
     calc {
-        m(b,s,n-s);
+         m(b,s,n-s);
       == { reveal m(); }
-        max(0, ceil((((n-s)-b) as real)/(s as real)));
+         max(0, ceil((((n-s)-b) as real)/(s as real)));
       == max(0, ceil((((n-b)-s) as real)/(s as real))); 
       == { reveal arith; }
-        max(0, ceil(((((n-b) as real)/(s as real)) - ((s/s) as real)) as real));
+         max(0, ceil(((((n-b) as real)/(s as real)) - ((s/s) as real)) as real));
       == max(0, ceil(((n-b) as real)/(s as real)) - 1);
       == { assert ceil(((n-b) as real)/(s as real)) - 1 >= 0; } 
-        ceil(((n-b) as real)/(s as real)) - 1;
+         ceil(((n-b) as real)/(s as real)) - 1;
       == { assert ceil(((n-b) as real)/(s as real)) > 0; }
-        max(0, ceil(((n-b) as real)/(s as real))) - 1;  
+         max(0, ceil(((n-b) as real)/(s as real))) - 1;  
       == { reveal m(); }
-        m(b,s,n) - 1;    
+         m(b,s,n) - 1;    
     }  
   }
 
@@ -381,7 +377,7 @@ module MasterLR {
   // ∃ d: ∀ n : S(n) <= d*n^k*sum_{i=0}^{m-1}a^i
   lemma {:axiom} lem_mmLR_SupBound(a:nat, b:nat, c:R0, s:nat, T:nat->R0, w:nat->R0, k:R0)  
     requires a > 0 && s > 0 && b >= s-1
-    requires bigOR0(w, n => powr(n as R0, k))
+    requires bigO(w, n => pow(n as R0, k))
     ensures exists d :: SupBoundPred(a, b, s, w, k, d)
 
 
@@ -397,17 +393,17 @@ module MasterLR {
   //          \ O(n^k*a^{n/b})    , a > 1
   lemma thm_masterMethodLR2(a:nat, b:nat, c:R0, T:nat->R0, w:nat->R0, k:R0)  
     requires a > 0 && b > 0
-    requires bigOR0(w, (n:nat) => powr(n as R0, k)) 
+    requires bigO(w, (n:nat) => pow(n as R0, k)) 
     requires forall n:nat :: T(n) == TbodyLR2(a, b, c, T, w, n) 
 
-    ensures a == 1 ==> bigOR0(T, (n:nat) => powr(n as R0, k + 1.0))
-    ensures a > 1  ==> bigOR0(T, (n:nat) => powr(n as R0, k)*powr(a as R0, (n/b) as R0))
+    ensures a == 1 ==> bigO(T, (n:nat) => pow(n as R0, k + 1.0))
+    ensures a > 1  ==> bigO(T, (n:nat) => pow(n as R0, k)*pow(a as R0, (n/b) as R0))
   {
     // proof using thm_masterMethodLR with s := b.
     assert a > 0;   
     assert b > 0;   
     assert b >= b - 1;
-    assert bigOR0(w, n => powr(n as R0, k));
+    assert bigO(w, n => pow(n as R0, k));
     assert forall n:nat :: T(n) == TbodyLR2(a, b, c, T, w, n); 
     assert forall n:nat :: T(n) == TbodyLR(a, b, c, b, T, w, n)
       by { reveal TbodyLR2, TbodyLR; } 
