theory/math/LemFunction.dfy
@@ -1,9 +1,27 @@
+include "./TypeR0.dfy"
 
 /**************************************************************************
   Functions
 **************************************************************************/
 
 module LemFunction {
+  import opened TypeR0
+
+  ghost function liftD<T>(f:nat->T, default:T) : int->T
+  {
+    k => if k < 0 then default else f(k as nat)
+  }
+
+  ghost function liftCi2r(f:int->int) : int->real
+  {
+    n => f(n) as real
+  }
+
+  // Lift f:nat->nat to f':nat->R0
+  ghost function liftToR0(f:nat->nat) : nat->R0
+  {
+    n => f(n) as R0
+  }
 
   lemma {:axiom} lem_funExt<A,B>(f1:A->B, f2:A->B)
     requires forall x:A :: f1(x) == f2(x)
