analysisByF/breakLinAVG.dfy
@@ -1,8 +1,8 @@
-include "../theory/math/SummationReal.dfy"
+include "../theory/math/SumReal.dfy"
 include "../theory/math/TypeR0.dfy"
 include "../theory/ComplexityR0.dfy"
 
-import opened SummationReal
+import opened SumReal
 import opened TypeR0
 import opened ComplexityR0
 
@@ -42,13 +42,13 @@ ghost method expectationLoop(N:nat)
   returns (tE:real)
   requires N > 0
   ensures tE == Tavg(N)
-  ensures tIsBigOR0(N, tE, n => n as R0)
+  ensures tIsBigO(N, tE, n => n as R0)
 {
   tE := 0.0; 
-  var p := 0; reveal sumr();  
+  var p := 0; reveal sum();  
   while p < N
     invariant 0 <= p <= N
-    invariant tE == sumr(0, p-1, i => (i+1) as real * (1.0 / N as real))
+    invariant tE == sum(0, p-1, i => (i+1) as real * (1.0 / N as real))
     decreases N - p
   {
     // Run the algorithm in scenario where P(p) holds
@@ -58,14 +58,14 @@ ghost method expectationLoop(N:nat)
     assert t == T(N,p);
     
     // Add weighted contribution to expectation
-    lem_sumr_dropLastAll(0, p-1);
+    lem_sum_dropLastAll(0, p-1);
     tE := tE + t as real * probability(N,pred,p);
     p  := p + 1;
   }
-  assert tE == sumr(0, N-1, i => (i+1) as real * (1.0 / N as real)); 
+  assert tE == sum(0, N-1, i => (i+1) as real * (1.0 / N as real)); 
   assert tE == Tavg(N) by { lem_solveSum(N); }
 
-  assert bigOR0(Tavg, n => n as R0) by { var c, n0 := lem_TavgBigOR0lin(); }
+  assert bigO(Tavg, n => n as R0) by { var c, n0 := lem_TavgBigOlin(); }
 }
 
 ghost function probability(N:nat, pred:nat->bool, p:nat) : R0
@@ -87,25 +87,25 @@ ghost method inputScenario(N:nat, p:nat) returns (pred0:nat->bool)
 
 lemma lem_solveSum(N:nat)
   requires N > 0
-  ensures Tavg(N) == sumr(0, N-1, i => (i+1) as real * (1.0 / N as real))
+  ensures Tavg(N) == sum(0, N-1, i => (i+1) as real * (1.0 / N as real))
 { 
   var c:real := 1.0 / N as real; 
   calc {
-       sumr(0, N-1, i => (i+1) as real * c);
+       sum(0, N-1, i => (i+1) as real * c);
     == { assert forall k:int :: 0<=k<=N-1 ==>   
            (i => (i+1) as real * c)(k) == (l => c*(i => (i+1) as real)(l))(k);
-         lem_sumr_leibniz(0, N-1, i => (i+1) as real * c, 
-                                  l => c*(i => (i+1) as real)(l)); }
-       sumr(0, N-1, l => c*(i => (i+1) as real)(l));
-    == { lem_sumr_linearityConst(0, N-1, c, i => (i+1) as real); }
-       c * sumr(0, N-1, i => (i+1) as real);
-    == { lem_sumr_shiftIndex(0, N-1, 1, i => (i+1) as real); }
-       c * sumr(1, N, i => (i => (i+1) as real)(i-1));
+         lem_sum_leibniz(0, N-1, i => (i+1) as real * c, 
+                                 l => c*(i => (i+1) as real)(l)); }
+       sum(0, N-1, l => c*(i => (i+1) as real)(l));
+    == { lem_sum_linearityConst(0, N-1, c, i => (i+1) as real); }
+       c * sum(0, N-1, i => (i+1) as real);
+    == { lem_sum_shiftIndex(0, N-1, 1, i => (i+1) as real); }
+       c * sum(1, N, i => (i => (i+1) as real)(i-1));
     == { assert forall k:int :: 1<=k<=N ==> 
            (i => ((i-1)+1) as real)(k) == (i => i as real)(k);
-         lem_sumr_leibniz(1, N, i => (i => (i+1) as real)(i-1), i => i as real); }
-       c * sumr(1, N, i => i as real);
-    == { lem_sumr_interval(1, N); }
+         lem_sum_leibniz(1, N, i => (i => (i+1) as real)(i-1), i => i as real); }
+       c * sum(1, N, i => i as real);
+    == { lem_sum_interval(1, N); }
        c * ((N*(N+1) + 1*(1-1)) as real / 2.0);
     == c * ((N*(N+1)) as real / 2.0);  
     == (1.0 / N as real) * ((N*(N+1)) as real / 2.0); 
@@ -113,8 +113,8 @@ lemma lem_solveSum(N:nat)
   }
 } 
 
-lemma lem_TavgBigOR0lin() returns (c:R0, n0:nat)
-  ensures bigOR0from(c, n0, Tavg, n => n as R0)
+lemma lem_TavgBigOlin() returns (c:R0, n0:nat)
+  ensures bigOfrom(c, n0, Tavg, n => n as R0)
 {
   // we show that c=1 and n0=1
   c, n0 := 1.0, 1;
