analysisByMM/quad.dfy
@@ -1,12 +1,12 @@
 include "../theory/math/ExpReal.dfy"
-include "../theory/math/Misc.dfy"
+include "../theory/math/LemFunction.dfy"
 include "../theory/math/TypeR0.dfy"
 include "../theory/ComplexityR0.dfy"
 include "../theory/GrowthRatesR0.dfy"
 include "../theory/MasterLR.dfy"
 
 import opened ExpReal
-import opened Misc
+import opened LemFunction
 import opened TypeR0
 import opened ComplexityR0
 import opened GrowthRatesR0
@@ -15,7 +15,7 @@ import opened MasterLR
 method quad(N:nat)
   returns (ghost t:nat, ghost t':nat)
   ensures t == T1(N, N)
-  ensures bigOR0(liftToR0(n => T1(n,N)), polyGrowthR0(2.0))
+  ensures bigO(liftToR0(n => T1(n,N)), polyGrowth(2.0))
 {
   var i, j; reveal T1(),T2();
   i, j, t, t' := 0, 0, 0, 0;
@@ -72,7 +72,7 @@ lemma lem_T2def(n:nat)
 }
 
 lemma lem_T1BigOquad(N:nat)
-  ensures bigOR0(liftToR0(n => T1(n,N)), n => powr(n as R0, 2.0))
+  ensures bigO(liftToR0(n => T1(n,N)), n => pow(n as R0, 2.0))
 {
   var a:nat       := 1;
   var b:nat       := 0;
@@ -89,13 +89,13 @@ lemma lem_T1BigOquad(N:nat)
     reveal TbodyLR; 
     lem_T1def(n, N);
   } 
-  assert bigOR0(w, n => powr(n as R0, k))
+  assert bigO(w, n => pow(n as R0, k))
    by { lem_T1BigOquadAux(N); }
   thm_masterMethodLR(a, b, c, s, T1', w, k); 
 }
 
 lemma {:isolate_assertions} lem_T1BigOquadAux(N:nat)
-  ensures bigOR0(liftToR0(n => T2(N)), n => powr(n as R0, 1.0))
+  ensures bigO(liftToR0(n => T2(N)), n => pow(n as R0, 1.0))
 {
   var k:R0 := 1.0;
   var w:nat->R0 := liftToR0(n => T2(N)); 
@@ -103,21 +103,21 @@ lemma {:isolate_assertions} lem_T1BigOquadAux(N:nat)
   var c:R0 := T2(N) as R0;
   var n0:nat := 1; 
   forall n:nat | 0 <= 1 <= n
-    ensures w(n) <= c * powr(n as R0, k) as R0
+    ensures w(n) <= c * pow(n as R0, k) as R0
   {
     assert T2(N) as R0 <= c * n as R0
       by { assert T2(N) <= (T2(N))*n; }
-    assert powr(n as R0, k) == n as R0 
-      by { assert n as R0 > 0.0; lem_powrOne(n as R0); }
-    assert T2(N) as R0 <= c * powr(n as R0, k); 
-    assert w(n) <= c * powr(n as R0, k)
+    assert pow(n as R0, k) == n as R0 
+      by { assert n as R0 > 0.0; lem_powOne(n as R0); }
+    assert T2(N) as R0 <= c * pow(n as R0, k); 
+    assert w(n) <= c * pow(n as R0, k)
       by { assert w(n) == T2(N) as R0; }
   }
-  assert bigOR0from(c, n0, w, n => powr(n as R0, k));  
+  assert bigOfrom(c, n0, w, n => pow(n as R0, k));  
 }
 
 lemma lem_T2BigOlin()
-  ensures bigOR0(liftToR0(T2), n => powr(n as R0, 1.0))
+  ensures bigO(liftToR0(T2), n => pow(n as R0, 1.0))
 {
   var a:nat       := 1;
   var b:nat       := 0;
@@ -133,15 +133,15 @@ lemma lem_T2BigOlin()
     reveal TbodyLR;
     lem_T2def(n);
   } 
-  assert bigOR0(w, n => powr(n as R0, k)) by {   
+  assert bigO(w, n => pow(n as R0, k)) by {   
     // we show that c=1 and n0=1
     forall n:nat | 0 <= 1 <= n
-      ensures w(n) <= 1.0*polyGrowthR0(k)(n)
+      ensures w(n) <= 1.0*polyGrowth(k)(n)
     {
-      assert powr(n as R0, k) == 1.0 by { lem_powrZeroAll(); }
-      assert w(n) <= 1.0*polyGrowthR0(k)(n); 
+      assert pow(n as R0, k) == 1.0 by { lem_powZeroAll(); }
+      assert w(n) <= 1.0*polyGrowth(k)(n); 
     }
-    assert bigOR0from(1.0, 1, w, polyGrowthR0(k));
+    assert bigOfrom(1.0, 1, w, polyGrowth(k));
   } 
   thm_masterMethodLR(a, b, c, s, T2', w, k);
 }
