analysisByMM/quadv2.dfy
@@ -1,12 +1,12 @@
 include "../theory/math/ExpReal.dfy"
-include "../theory/math/Misc.dfy"
+include "../theory/math/LemFunction.dfy"
 include "../theory/math/TypeR0.dfy"
 include "../theory/ComplexityR0.dfy"
 include "../theory/GrowthRatesR0.dfy"
 include "../theory/MasterLR.dfy"
 
 import opened ExpReal
-import opened Misc
+import opened LemFunction
 import opened TypeR0
 import opened ComplexityR0
 import opened GrowthRatesR0
@@ -15,10 +15,10 @@ import opened MasterLR
 method quad(N:nat)
   returns (ghost t:nat, ghost t':nat)
   ensures t == T1(N, N)  
-  //ensures bigOR0(liftToR0((n:nat) => T1(N,n)), polyGrowthR0(1.0))
-  ensures bigOR0(liftToR0((n:nat) => T1(N,n)), polyGrowthR0(2.0))
-  //ensures bigOR0(liftToR0((n:nat) => if n<=N then T1(N,N,n) else 0), polyGrowthR0(2.0))
-  //ensures bigOR0(liftToR0((n:nat) requires n<=N => T1(N,N,n)), polyGrowthR0(2.0))
+  //ensures bigO(liftToR0((n:nat) => T1(N,n)), polyGrowth(1.0))
+  ensures bigO(liftToR0((n:nat) => T1(N,n)), polyGrowth(2.0))
+  //ensures bigO(liftToR0((n:nat) => if n<=N then T1(N,N,n) else 0), polyGrowth(2.0))
+  //ensures bigO(liftToR0((n:nat) requires n<=N => T1(N,N,n)), polyGrowth(2.0))
 {
   var i, j; reveal T1(),T2(); //var M := N;
   i, j, t, t' := 0, 0, 0, 0;
@@ -92,7 +92,7 @@ lemma lem_T2def(M:nat, j:nat)
 
 // lemma {:isolate_assertions} lem_T1BigOquad(N:nat, M:nat)
 //   requires N == M
-//   ensures bigOR0(liftToR0((n:nat) => if n<=N then T1(N,N,n) else 0), n => powr0(n as R0, 2.0))
+//   ensures bigO(liftToR0((n:nat) => if n<=N then T1(N,N,n) else 0), n => pow(n as R0, 2.0))
 // {
 //   var a:nat       := 1;
 //   var b:nat       := 0;
@@ -186,7 +186,7 @@ lemma lem_T2def(M:nat, j:nat)
 // }
 
 lemma {:isolate_assertions} lem_T1BigOquad(N:nat)
-  ensures bigOR0(liftToR0((n:nat) => T1(N,n)), n => powr(n as R0, 2.0))
+  ensures bigO(liftToR0((n:nat) => T1(N,n)), n => pow(n as R0, 2.0))
 {
   var a:nat       := 1;
   var b:nat       := 0;
@@ -204,11 +204,11 @@ lemma {:isolate_assertions} lem_T1BigOquad(N:nat)
     lem_T1def(N, n);
   } 
 
-  assert bigOR0(w, n => powr(n as R0, k)) by {
+  assert bigO(w, n => pow(n as R0, k)) by {
     lem_T2BigOlin(N);
-    assert bigOR0(liftToR0(n => T2(N,n)), n => powr(n as R0, 1.0));
-    var c2:R0, n0:nat :| bigOR0from(c2, n0, liftToR0(n => T2(N,n)), n => powr(n as R0, 1.0));
-    assert forall n:nat :: 0 <= n0 <= n ==> liftToR0(n => T2(N,n))(n) <= c2*powr(n as R0, 1.0);
+    assert bigO(liftToR0(n => T2(N,n)), n => pow(n as R0, 1.0));
+    var c2:R0, n0:nat :| bigOfrom(c2, n0, liftToR0(n => T2(N,n)), n => pow(n as R0, 1.0));
+    assert forall n:nat :: 0 <= n0 <= n ==> liftToR0(n => T2(N,n))(n) <= c2*pow(n as R0, 1.0);
     
   }
     //by { lem_T2BigOlin(N, M); }
@@ -242,7 +242,7 @@ lemma {:isolate_assertions} lem_T1BigOquad(N:nat)
 
 
 lemma lem_T2BigOlin(N:nat)
-  ensures bigOR0(liftToR0(n => T2(N,n)), n => powr(n as R0, 1.0)) 
+  ensures bigO(liftToR0(n => T2(N,n)), n => pow(n as R0, 1.0)) 
 {
   var a:nat       := 1;
   var b:nat       := 0;
@@ -260,15 +260,15 @@ lemma lem_T2BigOlin(N:nat)
       lem_T2def(N,n); 
     //}
   } 
-  assert bigOR0(w, n => powr(n as R0, k)) by {   
+  assert bigO(w, n => pow(n as R0, k)) by {   
     // we show that c=1 and n0=1
     forall n:nat | 0 <= 1 <= n
-      ensures w(n) <= 1.0*polyGrowthR0(k)(n)
+      ensures w(n) <= 1.0*polyGrowth(k)(n)
     {
-      assert powr(n as R0, k) == 1.0 by { lem_powrZeroAll(); }
-      assert w(n) <= 1.0*polyGrowthR0(k)(n); 
+      assert pow(n as R0, k) == 1.0 by { lem_powZeroAll(); }
+      assert w(n) <= 1.0*polyGrowth(k)(n); 
     }
-    assert bigOR0from(1.0, 1, w, polyGrowthR0(k));
+    assert bigOfrom(1.0, 1, w, polyGrowth(k));
   } 
   thm_masterMethodLR(a, b, c, s, T2', w, k);
 }
