test/testMath.dfy
@@ -1,27 +1,33 @@
+include "../theory/math/SumInt.dfy"
+include "../theory/math/SumReal.dfy"
+include "../theory/math/SumSeqReal.dfy"
+include "../theory/math/SumSetReal.dfy"
 
-include "../theory/math.dfy"
-include "../theory/mathSum.dfy"
+import Int  = SumInt
+import Real = SumReal
+import SeqR = SumSeqReal
+import SetR = SumSetReal
 
 ghost method test_sumrInterval() {
-  reveal sumr();
-  var s := sumr(0, 2, x => 1.0);
+  reveal Real.sum();
+  var s := Real.sum(0, 2, x => 1.0);
   assert s == 3.0; 
 }
 
 ghost method test_sumInterval() {
-  reveal sum();
-  var s := sum(0, 2, x => 1);
+  reveal Int.sum();
+  var s := Int.sum(0, 2, x => 1);
   assert s == 3; 
 }
 
 ghost method test_sumSeq() {
-  reveal sumSeq();
-  var s := sumSeq([0,1,2], x => 1.0);
+  reveal SeqR.sum();
+  var s := SeqR.sum([0,1,2], x => 1.0);
   assert s == 3.0; 
 }
  
 ghost method test_sumSet() {
-  reveal sumSet();
-  var s2 := sumSet({0,1,2}, x => 1.0);
+  reveal SetR.sum();
+  var s2 := SetR.sum({0,1,2}, x => 1.0);
   // assert s2 == 3.0;  // not working
 }
