theory/math/SumReal.dfy
@@ -1,0 +1,230 @@
+
+/**************************************************************************
+  Sum over integer intervals and real codomain
+**************************************************************************/
+
+module SumReal {
+
+  // sum_{k=a}^{b}f(k)
+  opaque ghost function sum(a:int, b:int, f:int->real): real
+    decreases b - a
+  {
+    if a > b  
+    then 0.0
+    else f(a) + sum(a+1, b, f)
+  }
+
+  // a <= b+1 ==> sum_{k=a}^{b+1}f(k) = sum_{k=a}^{b}f(k) + f(b+1)
+  lemma lem_sum_dropLast(a:int, b:int, f:int->real)
+    requires a <= b+1
+    ensures  sum(a, b+1, f) == sum(a, b, f) + f(b+1) 
+    decreases b - a
+  { 
+    if a == b+1 {   
+      // BC: a > b
+      calc {
+          sum(b+1, b+1, f);
+        == { reveal sum(); }
+          f(b+1);
+        == 0.0 + f(b+1) ;
+        == { reveal sum(); }
+          sum(a, b, f) + f(b+1) ;       
+      }
+    } else {  
+      // Step. a <= j
+      //   IH: sum(a+1, b+1, f) = sum(a+1, b, f) + f(b+1)
+      //    T: sum(a, b+1, f)   = sum(a, b, f)   + f(b+1)
+      calc {  
+          sum(a, b+1, f);
+        == { reveal sum(); } 
+          f(a) + sum(a+1, b+1, f);
+        == { lem_sum_dropLast(a+1, b, f); }  // by IH
+          f(a) + (sum(a+1, b, f) + f(b+1));
+        == (f(a) + sum(a+1, b, f)) + f(b+1);
+        == { reveal sum(); }
+          sum(a, b, f) + f(b+1);           
+      }
+    }
+  } 
+
+  lemma lem_sum_dropLastAll(a:int, b:int)
+    requires a <= b+1
+    ensures  forall f:int->real :: sum(a, b+1, f) == sum(a, b, f) + f(b+1) 
+  { 
+    forall f:int->real
+      ensures sum(a, b+1, f) == sum(a, b, f) + f(b+1) 
+    {
+      lem_sum_dropLast(a, b, f);
+    }
+  }
+
+  // i <= j+1 ==> c*sum_{k=i}^{j}f(k) = sum_{k=i}^{j}c*f(k)
+  lemma lem_sum_linearityConst(a:int, b:int, c:real, f:int->real)
+    requires a <= b+1
+    ensures  c*sum(a, b, f) == sum(a, b, k => c*f(k))
+    decreases b - a
+  { 
+    if a == b+1 {   
+      // BC: a > b
+      calc {
+          c*sum(b+1, b, f);
+        == { reveal sum(); }
+          0.0;
+        == { reveal sum(); }
+          sum(b+1, b, k => c*f(k));       
+      }
+    } else {  
+      // Step. a <= b
+      //   IH: c*sum(a+1, b, f) = c*sum(a+1, b, k => c*f(k))
+      //    T: c*sum(a, b, f)   = c*sum(a, b, k => f(k))
+      calc {  
+          c*sum(a, b, f);
+        == { reveal sum(); } 
+          c*(f(a) + sum(a+1, b, f));
+        == c*f(a) + c*sum(a+1, b, f);         
+        == { lem_sum_linearityConst(a+1, b, c, f); }  // by IH
+          c*f(a) + sum(a+1, b, k => c*f(k)); 
+        == (k => c*f(k))(a) + sum(a+1, b, k => c*f(k));
+        == { reveal sum(); } 
+          sum(a, b, k => c*f(k));           
+      } 
+    }  
+  }
+
+  // a <= b+1 ==> sum_{k=a}^{b}c = c*(b - a + 1)
+  lemma lem_sum_const(a:int, b:int, c:real)
+    requires a <= b+1
+    ensures  sum(a, b, k => c) == c * (b - a + 1) as real
+    decreases b - a
+  { 
+    if a == b+1 {   
+      // BC: a > b
+      calc {
+          sum(b+1, b, k => c); 
+        == { reveal sum(); } 
+          0.0; 
+        == (b - (b+1) + 1) as real;
+      }
+    } else {  
+      // Step. a <= b
+      //   IH: sum(a+1, b, k => c) = c*(b - (a+1) + 1) = c*(b - a)
+      //    T: sum(a, b, k => c)   = c*(b - a + 1) 
+      calc {  
+          sum(a, b, k => c);
+        == { reveal sum(); }
+          c + sum(a+1, b, x => c);
+        == { lem_sum_const(a+1, b, c); }  // by IH
+          (c + c* (b - (a+1) + 1) as real);
+        == c + c*((b - a) as real);      
+        == c* (b - a + 1) as real;             
+      }
+    }
+  }
+
+  lemma lem_sum_constAll(a:int, b:int)
+    requires a <= b+1
+    ensures  forall c:real :: sum(a, b, k => c) == c * (b - a + 1) as real
+  { 
+    forall c:real
+      ensures sum(a, b, k => c) == c * (b - a + 1) as real
+    {
+      lem_sum_const(a, b, c);
+    }
+  } 
+
+  // a <= b+1 ==> sum_{k=a}^{b}f(k) = sum_{k=a+d}^{b+d}f(k-d)
+  lemma lem_sum_shiftIndex(a:int, b:int, d:int, f:int->real)
+    requires a <= b+1
+    ensures  sum(a, b, f) == sum(a+d, b+d, k => f(k-d))
+    decreases b - a
+  { 
+    if a == b+1 {   
+      // BC: a > b
+      calc {
+          sum(b+1, b, f);
+        == { reveal sum(); }
+          0.0;
+        == { reveal sum(); }
+          sum(b+1+d, b+d, k => f(k-d));       
+      }
+    } else {  
+      // Step. a <= b
+      //   IH: sum(a+1, b, f) = sum((a+d)+1, b+d, k => f(k-d))
+      //    T: sum(a, b, f)   = sum(a+d, b+d, k => f(k-d))
+      calc {  
+          sum(a, b, f);
+        == { reveal sum(); } 
+          f(a) + sum(a+1, b, f);
+        == { lem_sum_shiftIndex(a+1, b, d, f); }  // by IH
+          f(a) + sum(a+1+d, b+d, k => f(k-d));
+        == (k => f(k-d))(a+d) + sum((a+d)+1, b+d, k => f(k-d));
+        == { reveal sum(); }
+          sum(a+d, b+d, k => f(k-d));           
+      }
+    }
+  } 
+
+  // a <= b+1 ==> sum_{k=a}^{b}k = (b*(b+1) + a*(1-a))/2 
+  lemma lem_sum_interval(a:int, b:int)
+    requires a <= b+1 
+    decreases b - a
+    ensures sum(a, b, k => k as real) == (b*(b+1) + a*(1-a)) as real / 2.0
+  { 
+    if a == b+1 {   
+      // BC: a > b
+      calc {
+          sum(b+1, b, k => k as real);
+        == { reveal sum(); }
+          0.0;
+        == (b*(b+1) + ((b+1))*(1-((b+1)))) as real / 2.0;
+      }
+    } else {  
+      // Step. a <= b
+      //   IH: sumr(a+1, b, K => k) = (b*(b+1) + (a+1)*(1-(a+1)))/2 
+      //    T: sumr(a, b, k => k)   = (b*(b+1) + a*(1-a))/2 
+      calc {  
+          sum(a, b, k => k as real);
+        == { reveal sum(); }
+          a as real + sum(a+1, b, k => k as real);
+        == { lem_sum_interval(a+1, b); }  // by IH
+          a as real + (b*(b+1) + (a+1)*(1-(a+1))) as real / 2.0;
+        == (b*(b+1) + a*(1-a)) as real / 2.0;            
+      }
+    } 
+  }
+
+  // a <= b+1 /\ (∀ k : a<=k<=b : f(k) == g(k)) 
+  //          ==> sum_{k=a}^{b}f = sum_{k=a}^{b}g
+  lemma lem_sum_leibniz(a:int, b:int, f:int->real, g:int->real)
+    requires a <= b+1
+    requires forall k:int :: a<=k<=b ==> f(k) == g(k)
+    ensures sum(a, b, f) == sum(a, b, g)
+    decreases b - a
+  {
+    if a == b+1 {   
+      // BC: a > b
+      calc {
+          sum(b+1, b, f);
+        == { reveal sum(); }
+          0.0;
+        == { reveal sum(); }
+          sum(b+1, b, g);       
+      }
+    } else {  
+      // Step. a <= b
+      //   IH: sum(a+1, b, f) = sum(a+1, b, g)
+      //    T: sum(a, b, f)   = sum(a, b, g)
+      calc {  
+          sum(a, b, f);
+        == { reveal sum(); } 
+          f(a) + sum(a+1, b, f);
+        == g(a) + sum(a+1, b, f);
+        == { lem_sum_leibniz(a+1, b, f, g); }  // by IH
+          g(a) + sum(a+1, b, g);
+        == { reveal sum(); }
+          sum(a, b, g);           
+      }
+    }
+  } 
+
+}
