theory/math/SumSeqReal.dfy
@@ -1,0 +1,16 @@
+
+/**************************************************************************
+  Sum over integer sequences and real codomain
+**************************************************************************/
+
+module SumSeqReal {
+
+  opaque ghost function sum(s:seq<int>, f:int->real): real
+    decreases s
+  {
+    if |s| == 0 
+    then 0.0
+    else f(s[0]) + sum(s[1..], f)
+  }
+
+}
