theory/math/SumSetReal.dfy
@@ -1,0 +1,17 @@
+
+/**************************************************************************
+  Sum over integer sets and real codomain
+**************************************************************************/
+
+module SumSetReal {
+
+  opaque ghost function sum(s:set<int>, f:int->real): real
+    decreases s
+  {
+    if |s| == 0 
+    then 0.0
+    else var x :| x in s;
+        f(x) + sum(s - {x}, f)
+  }
+
+}
